Cleanup

src/lib/communication/DY.Lib.Communication.API.Lemmas.fst
@@ -23,10 +23,10 @@ val encrypt_message_proof:
   Lemma
   (requires
     has_communication_layer_invariants /\
-    is_knowable_by (join (principal_label sender) (principal_label receiver)) tr payload /\
     is_secret (long_term_key_label sender) tr nonce /\
     nonce `has_usage tr` PkNonce /\
     is_public_key_for tr pk_receiver (LongTermPkEncKey comm_layer_pkenc_tag) receiver /\
+    is_knowable_by (join (principal_label sender) (principal_label receiver)) tr payload /\
     event_triggered tr sender (CommConfSendMsg sender receiver payload)
   )
   (ensures
@@ -45,8 +45,8 @@ val send_confidential_proof:
     trace_invariant tr /\
     has_pki_invariant /\
     has_communication_layer_invariants /\
-    comm_layer_preds_later tr (higher_layer_preds.send_conf sender receiver payload) /\
     has_communication_layer_event_predicates higher_layer_preds /\
+    comm_layer_preds_later tr (higher_layer_preds.send_conf sender receiver payload) /\
     // We only require the payload to flow to the sender and receiver to allow
     // the sender to send a payload readable by other principals. If you want
     // the payload to be only readable by the sender and receiver, you can use
@@ -65,14 +65,14 @@ let send_confidential_proof #invs tr higher_layer_preds keys_sess_ids sender rec
     let (Some pk_receiver, tr) = get_public_key sender keys_sess_ids.pki (LongTermPkEncKey comm_layer_pkenc_tag) receiver tr in
     let (nonce, tr) = mk_rand PkNonce (long_term_key_label sender) 32 tr in
     let ((), tr) = trigger_event sender (CommConfSendMsg sender receiver payload) tr in
-    let msg_encrypted = encrypt_message pk_receiver nonce payload in
-    assert(higher_layer_preds.send_conf sender receiver payload tr);
     assert(event_triggered tr sender (CommConfSendMsg sender receiver payload));
     encrypt_message_proof tr sender receiver pk_receiver nonce payload;
+    let msg_encrypted = encrypt_message pk_receiver nonce payload in
     let (msg_id, tr) = send_msg msg_encrypted tr in
     assert(tr_out == tr);
     ()
   )
+
 
 val decrypt_message_proof:
   {|cinvs:crypto_invariants|} ->
@@ -102,7 +102,6 @@ let decrypt_message_proof #cinvs tr receiver sk_receiver msg_encrypted =
   | Some payload -> ()
   | _ -> ()
 
-
 val receive_confidential_proof:
   {|invs:protocol_invariants|} ->
   tr:trace ->
@@ -130,8 +129,8 @@ let receive_confidential_proof #invs tr higher_layer_preds comm_keys_ids receive
   | (Some payload, tr_out) -> (
     let (Some sk_receiver, tr) = get_private_key receiver comm_keys_ids.private_keys (LongTermPkEncKey comm_layer_pkenc_tag) tr in
     let (Some msg_encrypted, tr) = recv_msg msg_id tr in
-    let Some msg_plain = decrypt_message sk_receiver msg_encrypted in
     decrypt_message_proof tr receiver sk_receiver msg_encrypted;
+    let Some msg_plain = decrypt_message sk_receiver msg_encrypted in
     let ((), tr) = trigger_event receiver (CommConfReceiveMsg receiver payload) tr in
     assert(tr_out == tr);
     ()
@@ -183,6 +182,7 @@ let sign_message_proof #cinvs tr sender receiver payload is_encrypted sk_sender 
     serialize_wf_lemma signature_input (is_publishable tr) sig_input;
     let signature = sign sk_sender nonce sig_input_bytes in
     let msg_signed = {sender; receiver; payload; signature} in
+    assert(bytes_invariant tr signature);
     serialize_wf_lemma communication_message_sign (is_publishable tr) msg_signed;
     ()
   )
@@ -195,12 +195,11 @@ val send_authenticated_proof:
   sender:principal -> receiver:principal -> payload:bytes ->
   Lemma
   (requires
-    trace_invariant tr /\ has_private_keys_invariant /\
+    trace_invariant tr /\ 
+    has_private_keys_invariant /\
     has_communication_layer_invariants /\
-    //if_comm_conf_payload sender receiver payload tr /\
-    //comm_layer_preds_later tr (if_comm_conf_payload sender receiver payload) /\
-    comm_layer_preds_later tr (higher_layer_preds.send_auth sender payload) /\
     has_communication_layer_event_predicates higher_layer_preds /\
+    comm_layer_preds_later tr (higher_layer_preds.send_auth sender payload) /\
     is_publishable tr payload
   )
   (ensures (
@@ -214,9 +213,9 @@ let send_authenticated_proof #invs tr higher_layer_preds comm_keys_ids sender re
       let (Some sk_sender, tr) = get_private_key sender comm_keys_ids.private_keys (LongTermSigKey comm_layer_sign_tag) tr in
       let (nonce,  tr) = mk_rand SigNonce (long_term_key_label sender) 32 tr in      
       let ((), tr) = trigger_event sender (CommAuthSendMsg sender payload) tr in
-      assert(event_triggered tr sender (CommAuthSendMsg sender payload)); 
-      let msg_signed = sign_message sender receiver payload false sk_sender nonce in
+      assert(event_triggered tr sender (CommAuthSendMsg sender payload));
       sign_message_proof tr sender receiver payload false sk_sender nonce;
+      let msg_signed = sign_message sender receiver payload false sk_sender nonce in
       let (msg_id, tr) = send_msg msg_signed tr in
       assert(tr_out == tr);
       ()
@@ -265,48 +264,11 @@ let verify_message_proof #cinvs tr sender receiver msg_bytes is_encrypted vk_sen
   match verify_message receiver msg_bytes is_encrypted vk_sender with
   | Some {sender=sender'; receiver=receiver'; payload} -> (
     parse_wf_lemma communication_message_sign (is_publishable tr) msg_bytes;
-    //assert(is_publishable tr payload);
     let Some msg_signed = parse communication_message_sign msg_bytes in
-    
-    //assert(bytes_invariant tr vk_sender);
-    //assert(bytes_invariant tr msg_bytes);
-    //assert(bytes_invariant tr msg_signed.signature);
-    //normalize_term_spec bytes_invariant;
-    //reveal_opaque (`%verify) (verify);
-    
-
-    (*assert(event_triggered tr sender (CommAuthSendMsg sender payload) \/
-      get_signkey_label vk_sender `can_flow tr` public);
-    
-    let DY.Core.Bytes.Type.Sign sk nonce sig_input_bytes = msg_signed.signature in
-    assert(sign_pred.pred tr (Vk sk) sig_input_bytes \/
-      get_signkey_label vk_sender `can_flow tr` public);
-
-    assert(receiver == receiver');
-    assert(sender == sender' \/
-      get_signkey_label vk_sender `can_flow tr` public);*)
     
     if is_encrypted then (
       let sig_input_e = Encrypted {sender=sender'; receiver=msg_signed.receiver; payload=msg_signed.payload} in
-      //let sig_input_bytes_e = serialize signature_input #parseable_serializeable_bytes_signature_input sig_input_e in
       serialize_wf_lemma signature_input (is_publishable tr) sig_input_e;
-      //assert(verify vk_sender sig_input_bytes_e msg_signed.signature);      
-      //assert(bytes_invariant tr sig_input_bytes_e);      
-      //bytes_invariant_verify tr vk_sender sig_input_bytes_e msg_signed.signature;
-
-      (*let Some sig_input = parse signature_input sig_input_bytes in
-      assert(Encrypted? sig_input);
-      let sig_input_record = Encrypted?.msg sig_input in
-      assert(sign_pred.pred tr (Vk sk) sig_input_bytes \/
-        get_signkey_label vk_sender `can_flow tr` public);
-      assert(msg_signed.receiver == receiver);
-      let sig_input' = Encrypted {sender=sender'; receiver=msg_signed.receiver; payload=msg_signed.payload} in
-      let sig_input_bytes' = serialize signature_input sig_input' in
-      assert(verify vk_sender sig_input_bytes' msg_signed.signature);
-      assert(sig_input_record.sender == sender \/
-        get_signkey_label vk_sender `can_flow tr` public);
-      assert(event_triggered tr sender (CommConfSendMsg sender receiver msg) \/
-        get_signkey_label (Vk sk) `can_flow tr` public);*)
       ()
     ) else (
       let sig_input_p = Plain {sender=sender'; receiver=msg_signed.receiver; payload=msg_signed.payload} in
@@ -316,31 +278,6 @@ let verify_message_proof #cinvs tr sender receiver msg_bytes is_encrypted vk_sen
   )
   | _ -> ()
 
-(*val extract_data_from_msg_id:
-  tr:trace ->
-  comm_keys_ids:communication_keys_sess_ids ->
-  receiver:principal -> msg_id:timestamp ->
-  (principal -> principal -> bytes -> prop) ->
-  prop
-let extract_data_from_msg_id tr comm_keys_ids receiver msg_id fn =
-  match recv_msg msg_id tr with
-  | (None, tr) -> True
-  | (Some msg_signed, tr) -> (
-    match get_sender msg_signed with
-    | None -> True
-    | Some sender -> (
-      match get_public_key receiver comm_keys_ids.pki (Verify comm_layer_sign_tag) sender tr with
-      | (None, tr) -> True
-      | (Some vk_sender, tr) -> (
-        match verify_message receiver msg_signed false vk_sender with
-        | None -> True
-        | Some {sender=sender'; receiver=receiver'; payload} -> (
-          fn sender receiver payload
-        )
-      )
-    )
-  )*)
-
 val receive_authenticated_proof:
   {|invs:protocol_invariants|} ->
   tr:trace ->
@@ -349,27 +286,29 @@ val receive_authenticated_proof:
   receiver:principal -> msg_id:timestamp ->
   Lemma
   (requires
-    trace_invariant tr /\ has_pki_invariant /\
+    trace_invariant tr /\ 
+    has_pki_invariant /\
     has_communication_layer_invariants /\
     has_communication_layer_event_predicates higher_layer_preds
   )
   (ensures (
     match receive_authenticated comm_keys_ids receiver msg_id tr with
+    | (None, tr_out) -> trace_invariant tr_out
     | (Some {sender; receiver; payload}, tr_out) -> (
       trace_invariant tr_out /\
       event_triggered tr_out receiver (CommAuthReceiveMsg sender receiver payload)
     )
-    | (None, tr_out) -> trace_invariant tr_out
   ))
 let receive_authenticated_proof #invs tr higher_layer_preds comm_keys_ids receiver msg_id =
   match receive_authenticated comm_keys_ids receiver msg_id tr with
   | (None, tr_out) -> ()
   | (Some {sender=sender'; receiver=receiver'; payload}, tr_out) -> (
     let (Some msg_signed, tr) = recv_msg msg_id tr in
-    let Some msg = parse_sig_message msg_signed in
-    let (Some vk_sender, tr) = get_public_key receiver comm_keys_ids.pki (LongTermSigKey comm_layer_sign_tag) msg.sender tr in
-    verify_message_proof tr msg.sender receiver msg_signed false vk_sender;
-    let ((), tr) = trigger_event receiver (CommAuthReceiveMsg msg.sender receiver payload) tr in
+    let Some sender = get_sender msg_signed in
+    let (Some vk_sender, tr) = get_public_key receiver comm_keys_ids.pki (LongTermSigKey comm_layer_sign_tag) sender tr in
+    verify_message_proof tr sender receiver msg_signed false vk_sender;
+    let (Some cm) = verify_message receiver msg_signed false vk_sender in
+    let ((), tr) = trigger_event receiver (CommAuthReceiveMsg sender receiver cm.payload) tr in
     assert(tr_out == tr);
     ()
   )
@@ -385,13 +324,13 @@ val encrypt_and_sign_message_proof:
   Lemma
   (requires
     has_communication_layer_invariants /\
-    is_knowable_by (join (principal_label sender) (principal_label receiver)) tr payload /\
     is_secret (long_term_key_label sender) tr enc_nonce /\
     is_secret (long_term_key_label sender) tr sign_nonce /\
     enc_nonce `has_usage tr` PkNonce /\
     sign_nonce `has_usage tr` SigNonce /\
     is_public_key_for tr pk_receiver (LongTermPkEncKey comm_layer_pkenc_tag) receiver /\
     is_private_key_for tr sk_sender (LongTermSigKey comm_layer_sign_tag) sender /\
+    is_knowable_by (join (principal_label sender) (principal_label receiver)) tr payload /\
     event_triggered tr sender (CommConfSendMsg sender receiver payload) /\
     event_triggered tr sender (CommAuthSendMsg sender payload) /\
     event_triggered tr sender (CommConfAuthSendMsg sender receiver payload)
@@ -402,72 +341,9 @@ val encrypt_and_sign_message_proof:
 let encrypt_and_sign_message_proof #cinvs tr sender receiver payload pk_receiver sk_sender enc_nonce sign_nonce =
   encrypt_message_proof #cinvs tr sender receiver pk_receiver enc_nonce payload;
   let enc_payload = encrypt_message pk_receiver enc_nonce payload in
-  assert(get_label tr sk_sender == long_term_key_label sender);
-  assert(is_publishable tr enc_payload);
-  assert(enc_payload == encrypt_message pk_receiver enc_nonce payload);
-  assert(event_triggered tr sender (CommConfSendMsg sender receiver payload));
-  assert(event_triggered tr sender (CommAuthSendMsg sender payload));
-  assert(get_label tr payload `can_flow tr` (join (principal_label sender) (principal_label receiver)));
-  //normalize_term_spec pk_dec;
-  //normalize_term_spec pk_enc;
-  //normalize_term_spec get_sk_label;
-  //normalize_term_spec get_sk_usage;
-  //normalize_term_spec pk;
-
-  (*assert(match pk_receiver with
-  | DY.Core.Bytes.Type.Pk sk -> get_usage sk == PkKey comm_layer_pkenc_tag empty
-  | _ -> False);
-  assert(match pk_receiver with
-  | DY.Core.Bytes.Type.Pk sk -> get_label sk == principal_label receiver
-  | _ -> False);
-
-  assert(is_publishable tr enc_payload);
-
-  assert(enc_payload == pk_enc pk_receiver enc_nonce payload);
-
-  
-    
-  eliminate exists sk_receiver. get_label sk_receiver == principal_label receiver
-  returns exists sk_receiver. pk_dec sk_receiver (pk_enc pk_receiver enc_nonce payload) == Some payload
-  with _. (
-    pk_dec_enc sk_receiver enc_nonce payload;
-    assert(
-        pk_dec sk_receiver (pk_enc (pk sk_receiver) enc_nonce payload) == Some payload
-    );
-    assert(Some payload == decrypt_message sk_receiver enc_payload);
-    assert(exists plain_msg.
-      Some plain_msg == decrypt_message sk_receiver enc_payload
-    );
-    assert(exists plain_msg.
-      get_label plain_msg `can_flow tr` (join (principal_label sender) (principal_label receiver)));
-
-    
-
-    assert(has_communication_layer_invariants cinvs /\
-      is_publishable tr enc_payload /\
-      is_secret (principal_label sender) tr sign_nonce /\
-      SigNonce? (get_usage sign_nonce) /\
-      is_signature_key (SigKey comm_layer_sign_tag empty) (principal_label sender) tr sk_sender /\
-      (
-        if true then (
-          (exists sk_receiver plain_msg.
-            Some plain_msg == pk_dec sk_receiver enc_payload /\
-            get_label sk_receiver == principal_label receiver /\
-            event_triggered tr sender (CommConfSendMsg sender receiver plain_msg) /\
-            event_triggered tr sender (CommAuthSendMsg sender plain_msg) /\      
-            get_label plain_msg `can_flow tr` (join (principal_label sender) (principal_label receiver))
-          )
-        ) else (
-          event_triggered tr sender (CommAuthSendMsg sender payload)
-        )
-      ));
-    sign_message_proof tr sender receiver enc_payload true sk_sender sign_nonce;
-    ()
-  );*)
   pk_enc_extract_msg_enc_lemma pk_receiver enc_nonce payload enc_payload;
   sign_message_proof tr sender receiver enc_payload true sk_sender sign_nonce;
   ()
-
 
 val send_confidential_authenticated_proof:
   {|invs:protocol_invariants|} ->
@@ -481,10 +357,10 @@ val send_confidential_authenticated_proof:
     has_private_keys_invariant /\
     has_pki_invariant /\
     has_communication_layer_invariants /\
+    has_communication_layer_event_predicates higher_layer_preds /\
     comm_layer_preds_later tr (higher_layer_preds.send_conf sender receiver payload) /\
     comm_layer_preds_later tr (higher_layer_preds.send_auth sender payload) /\
     comm_layer_preds_later tr (higher_layer_preds.send_conf_auth sender receiver payload) /\
-    has_communication_layer_event_predicates higher_layer_preds /\
     is_knowable_by (join (principal_label sender) (principal_label receiver)) tr payload
   )
   (ensures (
@@ -533,10 +409,7 @@ val verify_and_decrypt_message_proof:
       (
         (
           sender' == sender /\
-          //event_triggered tr sender (CommAuthSendMsg sender payload) /\        
-          //event_triggered tr sender (CommConfSendMsg sender receiver payload) /\
-          event_triggered tr sender (CommConfAuthSendMsg sender receiver payload) ///\
-          //is_knowable_by (join (principal_label sender) (principal_label receiver)) tr payload
+          event_triggered tr sender (CommConfAuthSendMsg sender receiver payload)
         ) \/ (
           is_corrupt tr (long_term_key_label sender)
         )
@@ -549,90 +422,10 @@ let verify_and_decrypt_message_proof #cinvs tr sender receiver msg_encrypted_sig
   | Some {sender=sender'; receiver=receiver'; payload} -> (
     verify_message_proof tr sender receiver msg_encrypted_signed true vk_sender;
     let Some {sender=sender''; receiver=receiver''; payload=enc_payload} = verify_message receiver msg_encrypted_signed true vk_sender in    
-    assert(is_publishable tr enc_payload /\
-      (
-        (
-          sender' == sender /\
-          (
-            match pk_enc_extract_msg enc_payload with
-            | None -> False
-            | Some plain_payload -> (
-              vk_sender `has_signkey_usage tr` long_term_key_type_to_usage (LongTermSigKey comm_layer_sign_tag) sender /\     
-              get_label tr enc_payload `can_flow tr` public /\
-              event_triggered tr sender (CommConfAuthSendMsg sender receiver plain_payload)
-            )
-          )
-        ) \/ (
-          is_corrupt tr (long_term_key_label sender)
-          //get_label vk_sender `can_flow tr` public
-        )
-      )
-    );
-
     decrypt_message_proof tr receiver sk_receiver enc_payload;
     let Some payload' = decrypt_message sk_receiver enc_payload in
-    
-    //assert(pk_enc_extract_pk enc_payload == Some (DY.Core.Bytes.Type.Pk sk_receiver));
-    assert(payload == payload');
-    assert(exists sender.
-      is_knowable_by (join (principal_label sender) (principal_label receiver)) tr payload /\
-      (       
-        event_triggered tr sender (CommConfSendMsg sender receiver payload) \/
-        is_publishable tr payload
-      )
-    );
-    assert(exists sender. is_knowable_by (join (principal_label sender) (principal_label receiver)) tr payload);
-
-    assert(is_knowable_by (principal_label receiver) tr payload);
-  
     pk_enc_extract_msg_dec_lemma sk_receiver enc_payload payload;
-    assert(
-      match pk_enc_extract_msg enc_payload with
-      | Some plain_payload -> (
-        payload == plain_payload /\
-        event_triggered tr sender (CommConfAuthSendMsg sender receiver plain_payload)
-       
-      ) \/
-      is_corrupt tr (long_term_key_label sender));
-
     ()
-    (*introduce ~(is_corrupt tr (principal_label sender)) /\ ~(is_publishable tr payload) ==> event_triggered tr sender (CommConfSendMsg sender receiver payload)
-    with _. (
-      assert(exists payload. event_triggered tr sender (CommConfSendMsg sender receiver payload));
-      eliminate exists plain_msg. event_triggered tr sender (CommConfSendMsg sender receiver plain_msg)
-      returns event_triggered tr sender (CommConfSendMsg sender receiver payload)
-      with _. (
-        assert(
-          event_triggered tr sender (CommAuthSendMsg sender payload) /\
-          is_knowable_by (join (principal_label sender) (principal_label receiver)) tr payload /\
-          event_triggered tr sender (CommConfSendMsg sender receiver payload)
-        );
-        ()
-      )
-    )*)
-    (*reveal_opaque (`%pk_enc) (pk_enc);
-    reveal_opaque (`%pk_dec) (pk_dec);
-    let DY.Core.Bytes.Type.PkEnc pk nonce msg = enc_payload in
-    assert(if_comm_conf_payload sender receiver'' enc_payload tr \/
-      is_corrupt tr (principal_label sender));
-    assert(get_usage sk_receiver == PkKey comm_layer_pkenc_tag empty);
-    assert(Pk sk_receiver == pk);
-    reveal_opaque (`%get_sk_usage) (get_sk_usage);
-    assert(get_sk_usage pk == PkKey comm_layer_pkenc_tag empty);
-    assert(
-      (
-        get_sk_label pk == principal_label receiver'' /\
-        event_triggered tr sender (CommConfSendMsg sender receiver'' msg)
-      ) \/
-        is_corrupt tr (principal_label sender)                                                        
-    );
-    assert(get_label sk_receiver == principal_label receiver);
-    assert(get_sk_label pk == principal_label receiver'' \/
-      is_corrupt tr (principal_label sender));
-    reveal_opaque (`%get_sk_label) (get_sk_label);
-    assert(receiver == receiver'' \/
-      is_corrupt tr (principal_label sender));
-    decrypt_message_proof tr receiver sk_receiver enc_payload;*)
   )
 
 val receive_confidential_authenticated_proof:
@@ -665,15 +458,11 @@ let receive_confidential_authenticated_proof #invs tr higher_layer_preds comm_ke
   | (None, tr_out) -> ()
   | (Some {sender; receiver=receiver'; payload}, tr_out) -> (
     let (Some msg_encrypted_signed, tr) = recv_msg msg_id tr in
-    let Some msg_sig = parse_sig_message msg_encrypted_signed in
+    let Some sender = get_sender msg_encrypted_signed in
     let (Some sk_receiver, tr) = get_private_key receiver comm_keys_ids.private_keys (LongTermPkEncKey comm_layer_pkenc_tag) tr in
-    let (Some vk_sender, tr) = get_public_key receiver comm_keys_ids.pki (LongTermSigKey comm_layer_sign_tag) msg_sig.sender tr in
-    let Some msg = verify_and_decrypt_message receiver msg_encrypted_signed sk_receiver vk_sender in
+    let (Some vk_sender, tr) = get_public_key receiver comm_keys_ids.pki (LongTermSigKey comm_layer_sign_tag) sender tr in
     verify_and_decrypt_message_proof tr sender receiver msg_encrypted_signed sk_receiver vk_sender;
-    assert(event_triggered tr sender (CommConfAuthSendMsg sender receiver payload) \/
-      is_corrupt tr (long_term_key_label sender));
-    assert(is_knowable_by (join (principal_label sender) (principal_label receiver)) tr msg.payload \/
-      is_corrupt tr (long_term_key_label sender));
+    let Some msg = verify_and_decrypt_message receiver msg_encrypted_signed sk_receiver vk_sender in
     let ((), tr) = trigger_event receiver (CommConfAuthReceiveMsg msg.sender receiver msg.payload) tr in
     assert(event_triggered tr receiver (CommConfAuthReceiveMsg msg.sender receiver msg.payload));
     assert(trace_invariant tr);
